# TD2 Robotique #

## Cinematique directe Theorie ##

**P1 : **
- **x1** = L1 \* cos(&theta;1)
- **y1** = L1 \* sin (&theta;1)
- **z1** = 0

**P2 :** 
- **x2** = x1 + L2 \* cos(&theta;2) \* cos(&theta;1)
- **y2** = y1 + L2 \* cos(&theta;2) \* sin(&theta;1)
- **z2 **= z1 + L2 \* sin(&theta;2)


**P2 : (absolue)** 
- **x2** = cos(&theta;1) \* ( L1 + L2 \* cos(&theta;2) )
- **y2** = sin (&theta;1) \* ( L1 + L2 \* cos(&theta;2) )
- **z2 **= L2 \* sin(&theta;2)

**P3 :** 
- **x3** = x2 + L3 \* cos(&theta;2 + &theta;3) \* cos(&theta;1)
- **y3** = y2 + L3 \* cos(&theta;2 + &theta;3) \* sin(&theta;1)
- **z3** = z2 + L3 \* sin(&theta;2 + &theta;3)

**P3 (absolue) :**
- **x3 **= cos(&theta;1) \* ( L1 + L2 \* cos(&theta;2) + L3 \* cos(&theta;2 + &theta;3) )
- **y3** = sin(&theta;1) \* ( L1 + L2 \* cos(&theta;2) + L3 \* cos(&theta;2 + &theta;3) )
- **z3** = L2 \* sin(&theta;2) + L3 \* sin(&theta;2 + &theta;3)

## Cinematique Directe Pratique ##

**P1 :** No change

**P2 :**  
- **n_x2** = x2 - (L2 \* (1 - cos(&alpha;))) \* cos(&theta;1)
- **n_y2** = y2 - (L2 \* (1 - cos(&alpha;))) \* sin(&theta;1)
- **n_z2** = z2 - (L2 \* sin(&alpha;))

**P2 (absolue) :**  
- **n_x2** = cos(&theta;1) \* ( L1 + L2 \* cos(&theta;2) ) - (L2 \* (1 - cos(&alpha;))) \* cos(&theta;1)
- **n_y2** = sin (&theta;1) \* ( L1 + L2 \* cos(&theta;2) ) - (L2 \* (1 - cos(&alpha;))) \* sin(&theta;1)
- **n_z2** = L2 \* sin(&theta;2) - (L2 \* sin(&alpha;))

**P3 :**  
- **n_x3** = n_x2 + L3 \* cos(&theta;2 + &theta;3) \* cos(&theta;1) - (L3 \* (1 - sin(&alpha;))) \* cos(&theta;1)
- **n_y3** = n_y2 + L3 \* cos(&theta;2 + &theta;3) \* sin(&theta;1) - (L3 \* (1 - sin(&alpha;))) \* sin(&theta;1)
- **n_z3** = n_z2 + L3 \* sin(&theta;2 + &theta;3) - (L3 \* cos(&alpha;))

**P3 (absolue) :**
- **n_x3** = cos(&theta;1) \* ( L1 + L2 \* cos(&theta;2) + L3 \* cos(&theta;2 + &theta;3) ) - (L2 \* (1 - cos(&alpha;))) \* cos(&theta;1) - (L3 \* (1 - sin(&alpha;))) \* cos(&theta;1)
- **n_y3** = sin(&theta;1) \* ( L1 + L2 \* cos(&theta;2) + L3 \* cos(&theta;2 + &theta;3) ) - (L2 \* (1 - cos(&alpha;))) \* sin(&theta;1) - (L3 \* (1 - sin(&alpha;))) \* sin(&theta;1)
- **n_z3** = L2 \* sin(&theta;2) + L3 \* sin(&theta;2 + &theta;3) - (L2 \* sin(&alpha;))  - (L3 \* cos(&alpha;))